src/theory.lean
@@ -9,7 +9,7 @@ def theory (L : language) := set (formula L)
 
 notation `theory `L:max := set (formula L)
 
-def theory.sf (T : theory L) : theory L := {p | ∃ q : formula L, q ∈ T ∧ p = q.sf}
+def theory.sf (T : theory L) : theory L := {p | ∃ q : formula L, q ∈ T ∧ p = q^1}
 
 prefix `⇑`:max := theory.sf
 
@@ -22,7 +22,7 @@ instance sf_itr_pow : has_pow (theory L) ℕ := ⟨theory.sf_itr⟩
 @[simp] lemma theory.sf_itr_0 (T : theory L) : T^0 = T := rfl
 @[simp] lemma theory.sf_itr_succ (T : theory L) (n) : T^(n+1) = ⇑(T^n) := rfl
 
-lemma theory.sf_itr_add (T : theory L) (i j : ℕ) : (T^i)^j = T^(i + j) :=
+lemma theory.pow_add (T : theory L) (i j : ℕ) : (T^i)^j = T^(i + j) :=
 by { induction j with j IH; simp[←nat.add_one, ←add_assoc], simp[IH] }
 
 inductive theory.add (T : theory L) (p : formula L) : theory L 
@@ -36,13 +36,15 @@ class closed_theory (T : theory L) := (cl : ∀ {p}, p ∈ T → sentence p)
 class extend (T₀ T : theory L) := (ss : T₀ ⊆ T)
 
 def proper_at (n : ℕ) (T : theory L) : Prop := ∀ (p : formula L) (s), p ∈ T → p.rew (s^n) ∈ T
+def proper'_at (n : ℕ) (T : theory L) : Prop := ∀ (p : formula L) (s : ℕ → term L),
+  p ∈ T → p.rew (λ x, if x < n then #x else s (x - n)) ∈ T
 
-def ordered_p (T : theory L) : Prop := ∀ (p : formula L), p ∈ T → p.sf ∈ T
+def ordered_p (T : theory L) : Prop := ∀ (p : formula L), p ∈ T → p^1 ∈ T
 
 class ordered (T : theory L) := (ordered : ordered_p T)
 
 lemma oedered_p_theory_sf (T : theory L) : ordered_p T → ordered_p ⇑T := λ h p hyp,
-by { rcases hyp with ⟨p', hyp_p, rfl⟩, refine ⟨p'.sf, _, rfl⟩, exact h _ hyp_p }
+by { rcases hyp with ⟨p', hyp_p, rfl⟩, refine ⟨p'^1, _, rfl⟩, exact h _ hyp_p }
 
 instance ordered_theory_sf {T : theory L} [od : ordered T] :
   ordered ⇑T := ⟨oedered_p_theory_sf _ od.ordered⟩
@@ -52,12 +54,19 @@ instance ordered_theory_sf_itr {T : theory L} [od : ordered T] : ∀ n : ℕ, or
 | (n+1) := @fopl.ordered_theory_sf _ _  (ordered_theory_sf_itr n)
 
 class proper (n : ℕ) (T : theory L) := (proper : proper_at n T)
+class proper' (n : ℕ) (T : theory L) := (proper : proper'_at n T)
 
 instance ordered_proper {T : theory L} [pp : proper 0 T] : ordered T :=
 ⟨λ p h, by { have := pp.proper, exact this _ (λ x, #(x+1)) h }⟩
 
+instance ordered_proper' {T : theory L} [pp : proper' 0 T] : ordered T :=
+⟨λ p h, by { have := pp.proper, exact this _ (λ x, #(x+1)) h }⟩
+
 lemma proper.proper0 {T : theory L} [proper 0 T] :
   ∀ {p : formula L} {s}, p ∈ T → p.rew s ∈ T := @proper.proper _ 0 T _
+
+lemma proper'.proper0 {T : theory L} [proper' 0 T] :
+  ∀ {p : formula L} {s}, p ∈ T → p.rew s ∈ T := @proper'.proper _ 0 T _
 
 instance : closed_theory (∅ : theory L) := ⟨λ _ h, by exfalso; exact h⟩
 
@@ -70,15 +79,13 @@ def openform : theory L := {p | p.Open = tt}
 instance (n) : proper n (openform : theory L) :=
 ⟨λ p s h, by { induction p; simp[openform] at*; simp* at* }⟩
 
-lemma theory_sf_itr_eq {T : theory L} : ∀ {n},
-  T^n = {p | ∃ q : formula L, q ∈ T ∧ p = q.sf_itr n}
-| 0      := by simp[formula.sf_itr]
-| (n+1)  := by { simp[@theory_sf_itr_eq n, theory.sf, formula.sf_itr], ext p,
+lemma theory_sf_itr_eq {T : theory L} : ∀ {i : ℕ},
+  T^i = {p | ∃ q : formula L, q ∈ T ∧ p = q^i}
+| 0      := by simp
+| (i+1)  := by { simp[@theory_sf_itr_eq i, theory.sf], ext p,
   simp, refine ⟨λ h, _, λ h, _⟩,
-  { rcases h with ⟨q1, ⟨q2, h, rfl⟩, rfl⟩, refine ⟨q2, h, _⟩,
-    simp[formula.sf, formula.nested_rew, add_assoc] },
-  { rcases h with ⟨q, h, rfl⟩, refine ⟨q.rew (λ x, #(x + n)), ⟨q, h, rfl⟩, _⟩,
-    simp[formula.sf, formula.nested_rew, add_assoc] } }
+  { rcases h with ⟨q1, ⟨q2, h, rfl⟩, rfl⟩, refine ⟨q2, h, by simp[formula.pow_add]⟩ },
+  { rcases h with ⟨q, h, rfl⟩, refine ⟨q^i, ⟨q, h, rfl⟩, by simp[formula.pow_add]⟩ } }
 
 lemma sentence_mem_theory_sf_itr {T : theory L} {p : formula L} (a : sentence p) (n : ℕ) :
   p ∈ T → p ∈ T^n := λ h,
@@ -95,36 +102,48 @@ begin
   intros n m p h,
   induction m with m IH, { exact h },
   { suffices : p ∈ T^(n + m), from IH this, simp[theory_sf_itr_eq] at h ⊢, rcases h with ⟨q, h, rfl⟩,
-    have := @proper.proper _ 0 T _ _ shift h,
-    refine ⟨q.sf, this, _⟩,
-    simp[formula.sf_itr, formula.sf, formula.nested_rew, nat.succ_add_eq_succ_add, ←add_assoc] }
+    have : q^1 ∈ T, from @proper.proper _ 0 T _ _ (λ x, #(x + 1)) h,
+    refine ⟨q^1, this, _⟩,
+    simp[formula.pow_add, formula.nested_rew, nat.succ_add_eq_succ_add, ←add_assoc] }
+end
+
+lemma proper'_sf_inclusion (T : theory L) [proper' 0 T] : ∀ {n m : ℕ} (h : n ≤ m),
+  T^m ⊆ T^n :=
+begin
+  suffices : ∀ {n m : ℕ}, T^(n+m) ⊆ T^n,
+  { intros n m eqn p hyp, have e : m = n + (m - n), exact (nat.add_sub_of_le eqn).symm, 
+    rw e at hyp,
+    exact this hyp },
+  intros n m p h,
+  induction m with m IH, { exact h },
+  { suffices : p ∈ T^(n + m), from IH this, simp[theory_sf_itr_eq] at h ⊢, rcases h with ⟨q, h, rfl⟩,
+    have : q^1 ∈ T, from @proper'.proper _ 0 T _ _ (λ x, #(x + 1)) h,
+    refine ⟨q^1, this, _⟩,
+    simp[formula.pow_add, formula.nested_rew, nat.succ_add_eq_succ_add, ←add_assoc] }
 end
 
 lemma ordered_inclusion (T : theory L) [ordered T] : ⇑T ⊆ T := λ p h,
 by { rcases h with ⟨p, hyp, rfl⟩, exact ordered.ordered _ hyp }
 
-lemma formula.sf_rew_sf_eq (s) (p : formula L) : p.sf.rew (s^1) = (p.rew s).sf :=
-by { simp[formula.sf, formula.nested_rew] }
-
 lemma proper_theory_sf_itr {n : ℕ} {T : theory L} (pp : proper_at n T) : ∀ m,
   proper_at (n+m) (T^m)
 | 0     := by { simp, exact @pp }
 | (m+1) := λ p s h, by { rcases h with ⟨p, hyp_p, rfl⟩, rw ←add_assoc,
-     show p.sf.rew ((s^(n + m))^1) ∈ ⇑(T^m), simp[formula.sf_rew_sf_eq],
+     show (p^1).rew ((s^(n + m))^1) ∈ ⇑(T^m), simp[←formula.pow_rew_distrib],
      refine ⟨p.rew (s^(n+m)), proper_theory_sf_itr m _ s hyp_p, rfl⟩ }
 
 instance properc_theory_sf_itr {T : theory L} [pp : proper 0 T] {n} :
-  proper n (T^n) := ⟨by { have := proper_theory_sf_itr pp.proper n, simp* at* }⟩ 
+  proper n (T^n) := ⟨by { have := proper_theory_sf_itr pp.proper n, simp* at* }⟩  
 
 lemma closed_proper {T : theory L} [cl : closed_theory T] : proper_at 0 T :=
 λ p s h, by { simp[@closed_theory.cl _ _ cl _ h], exact h }
 
 @[simp] lemma closed_theory_sf_eq {T : theory L} [cl : closed_theory T] : ⇑T = T :=
 by { ext p, refine ⟨λ hyp, _, λ hyp, _⟩, rcases hyp with ⟨p, hyp_p, rfl⟩,
-     simp[formula.sf, formula.sentence_rew (closed_theory.cl hyp_p), hyp_p],
+     simp[closed_theory.cl hyp_p, hyp_p],
      rw ← (formula.sentence_sf (closed_theory.cl hyp)), refine ⟨p, hyp, rfl⟩ }
 
-lemma sf_dsb (T : theory L) (p : formula L) : ⇑T+{p.sf} = ⇑(T+{p}) :=
+lemma sf_dsb (T : theory L) (p : formula L) : ⇑T+{p^1} = ⇑(T+{p}) :=
 begin
   ext x, split; intros h,
   { cases h with h hx, refine ⟨p, theory.add.new, rfl⟩,
