src/semantics.lean
@@ -31,7 +31,7 @@ instance (M : model L) : inhabited M.dom := ⟨M.one⟩
 | e (t =̇ u)        := t.val e = u.val e
 | e (p →̇ q)       := p.val e → q.val e
 | e (¬̇p)           := ¬(p.val e)
-| e (∀̇p)           := ∀ d : M.dom, (p.val (d ^ˢ e))
+| e (∀̇p)           := ∀ d : M.dom, (p.val (d ⌢ e))
 
 notation M` ⊧[`:80 e`] `p :50 := @formula.val _ M e p
 
@@ -48,8 +48,8 @@ lemma rew_val_eq : ∀ (s : ℕ → term L) {n} (t : vecterm L n) (e : ℕ → |
 | _ _ (vecterm.const c)  _ := rfl 
 | _ _ (vecterm.app f v)  _ := by simp[vecterm.rew, rew_val_eq _ v]
 
-@[simp] lemma sf_slide_val {n} (t : vecterm L n) : ∀ (e : ℕ → |M|) d, t.sf.val (d ^ˢ e) = t.val e :=
-by induction t; simp[slide]; simp*
+@[simp] lemma pow_val_concat {n} (t : vecterm L n) : ∀ (e : ℕ → |M|) d, (t^1).val (d ⌢ e) = t.val e :=
+by { induction t; simp[concat] at*; simp* }
 
 lemma rew_val_iff : ∀ (s : ℕ → term L) (p : formula L) (e : ℕ → |M|),
   (p.rew s).val e ↔ p.val (λ n, (s n).val e)
@@ -59,26 +59,26 @@ lemma rew_val_iff : ∀ (s : ℕ → term L) (p : formula L) (e : ℕ → |M|),
 | _ (p →̇ q)       _ := by simp[formula.rew, rew_val_iff _ p, rew_val_iff _ q]
 | _ (¬̇p)           _ := by simp[formula.rew, rew_val_iff _ p]
 | s (∀̇p)           e := by { simp[formula.rew, rew_val_iff _ p], refine forall_congr (λ d, _),
-    have : (λ n, (vecterm.val (d ^ˢ e) (s^1 $ n)).head) = (d ^ˢ λ n, ((s n).val e)),
-    { funext n,cases n; simp[slide, term.val, vecterm.val] },
+    have : (λ n, (vecterm.val (d ⌢ e) (s^1 $ n)).head) = (d ⌢ λ n, ((s n).val e)),
+    { funext n, cases n; simp[concat, term.val, vecterm.val], exact pow_val_concat _ _ _ },
     simp[this] }
 
-@[simp] lemma sf_slide_val_iff : ∀ (p : formula L) (e : ℕ → |M|) d, p.sf.val (d ^ˢ e) = p.val e
+@[simp] lemma pow_val_concat_iff : ∀ (p : formula L) (e : ℕ → |M|) d, (p^1).val (d ⌢ e) = p.val e
 | (formula.const c) _ _ := rfl
 | (formula.app p v) _ _ := by simp
 | (t =̇ u)        _ _ := by simp[term.val]
-| (p →̇ q)       _ _ := by simp[sf_slide_val_iff p, sf_slide_val_iff q]
-| (¬̇p)           _ _ := by simp[sf_slide_val_iff p]
-| (∀̇p)           e d₀ := by {intros, simp, simp[formula.sf,rew_val_iff], apply forall_congr,
+| (p →̇ q)       _ _ := by simp[pow_val_concat_iff p, pow_val_concat_iff q]
+| (¬̇p)           _ _ := by simp[pow_val_concat_iff p]
+| (∀̇p)           e d₀ := by {intros, simp, simp[formula.pow_eq, rew_val_iff], apply forall_congr,
     intros d,
-    have : (λ n, (vecterm.val (d ^ˢ d₀ ^ˢ e) ((λ x, #(x + 1))^1 $ n)).head) = (d ^ˢ e),
-    { ext n, cases n; simp }, simp[this] }
+    have : (λ n, (vecterm.val (d ⌢ d₀ ⌢ e) ((λ x, #(x + 1))^1 $ n)).head) = (d ⌢ e),
+    { ext n, cases n; simp[concat] }, simp[this] }
 
 private lemma modelsth_sf {T} : M ⊧ₜₕ T → M ⊧ₜₕ ⇑T := λ h p hyp_p e,
-by { rcases hyp_p with ⟨p, hyp_p', rfl⟩, simp[formula.sf, rew_val_iff],
+by { rcases hyp_p with ⟨p, hyp_p', rfl⟩, simp[formula.pow_eq, rew_val_iff],
      refine h _ hyp_p' _ }
 
-@[simp] lemma models_ex {p} {e : ℕ → |M|} : (∃̇p).val e ↔ ∃ d, p.val (d ^ˢ e) :=
+@[simp] lemma models_ex {p} {e : ℕ → |M|} : (∃̇p).val e ↔ ∃ d, p.val (d ⌢ e) :=
 by simp[formula.ex, models, rew_val_iff]
 
 @[simp] lemma models_and {p q} {e : ℕ → |M|} : (p ⩑ q).val e ↔ (p.val e ∧ q.val e) :=
@@ -109,8 +109,8 @@ begin
   { intros M hyp_T e h₁, simp[formula.val], contrapose, exact h₁ },
   case fopl.provable.q1 : T p t
   { intros M hyp_T e h, simp[rew_val_iff] at h ⊢,
-    have : (λ n, (vecterm.val e (ₛ[t] n)).head) = (t.val e) ^ˢ e,
-    { funext n, cases n; simp[slide, term.val, vecterm.val] },
+    have : (λ n, (vecterm.val e (ι[0 ⇝ t] n)).head) = (t.val e) ⌢ e,
+    { funext n, cases n; simp[term.val, vecterm.val, concat] },
     rw this, exact h _ },
   case fopl.provable.q2 : T p q
   { intros M hyp_T e h₁ h₂ d, exact (h₁ d) (h₂ d) },
@@ -152,9 +152,9 @@ lemma eval_iff : ∀ {p : formula L} {e₁ e₂ : ℕ → |M|},
 | (¬̇p)           e₁ e₂ a := by { simp[sentence, formula.arity] at*,
     simp[eval_iff a] }
 | (∀̇p)           e₁ e₂ a := by { simp[sentence, formula.arity] at*,
-    have : ∀ (d : |M|), p.val (d ^ˢ e₁) ↔ p.val (d ^ˢ e₂),
+    have : ∀ (d : |M|), p.val (d ⌢ e₁) ↔ p.val (d ⌢ e₂),
     { intros d, refine eval_iff (λ n eqn, _),
-      cases n, { simp }, simp, refine a _ (nat.lt_sub_right_of_add_lt eqn) },
+      cases n; simp[concat], refine a _ (nat.lt_sub_right_of_add_lt eqn) },
     exact forall_congr this }
 
 lemma eval_sentence_iff {p : formula L} {e : ℕ → |M|} (a : sentence p) : M ⊧[e] p ↔ M ⊧ p :=
@@ -165,7 +165,7 @@ lemma eval_sentence_iff {p : formula L} {e : ℕ → |M|} (a : sentence p) : M �
 lemma nfal_models_iff : ∀ {n} {p : formula L}, M ⊧ p ↔ M ⊧ nfal p n
 | 0     _ := iff.rfl
 | (n+1) p := by { simp[@nfal_models_iff n p], refine ⟨λ h e d, h _, λ h e, _⟩,
-  have : (e 0) ^ˢ (λ x, e (x + 1)) = e, { ext x, cases x; simp },
+  have : ((e 0) ⌢ λ x, e (x + 1) )= e, { ext x, cases x; simp[concat] },
   have := h (λ x, e (x + 1)) (e 0), simp* at * }
 
 end fopl
